We are working with the following lines
---

Line #1: $y = -\frac{1}{2}x + 13$

Line #2: $y = -x$

Line #3: $y = -3x + 28$

Line #4: $y = \frac{1}{4}x + 2$

Line #5: $y = x + 8$

Line #6: $y = 3$

Line #7: $y = \frac{3}{2}x + 3$

Line #8: $y = 12x - 28$

Line #9: $y = 2x - 19$

Line #10: $y = -2x + 11$


Find the intersection of Line #1 & Line #2 using substitution
---

Line #1: $y = -\frac{1}{2}x + 13$

Line #2: $y = -x$

Substitute $y$ from the equation for line #2 into the equation for line #1: $$-x = y = -\frac{1}{2}x + 13$$

Add $x$ to both sides:
$$0 = \frac{1}{2}x + 13$$

Subtract $13$ from both sides:
$$-13 = \frac{1}{2}x$$

Multiply both sides by $2$:
$$x = -26$$

Now insert $x = -26$ into the equation for line #2:
$$y = -(-26)$$
$$y = 26$$

So the intersection point is $(-26, 26)$


Find the intersection of Line #1 & Line #2 using elimination
---

Line #1: $y = -\frac{1}{2}x + 13$

Line #2: $y = -x$

Add $(-1)$ times line #2 to line #1:

$$y = -\frac{1}{2}x + 13$$
$$-y = x$$
$$0 = \frac{1}{2}x + 13$$

Multiply both sides by 2:
$$0 = x + 26$

Subtract $26$ from both sides
$$-26 = x$$

Then substitute $x = -26$ into the equation for line #2:
$$y = -(-26)$$
$$y = 26$$

So the intersection point is $(-26, 26)$


Find the intersection of Line #3 & Line #4 using substitution
---

Line #3: $y = -3x + 28$

Line #4: $y = \frac{1}{4}x + 2$

Substitute value for $y$ from the equation for line #4 into equation for line #3:
$$\frac{1}{4}x + 2 = -3x + 28$$

Add $3x$ to both sides:
$$3\frac{1}{4}x + 2 = 28$$

Subtract $2$ from both sides:
$$3\frac{1}{4}x = 26$$

Multipy both sides by $4$:
$$13x = 104$$

Divide both sides by $13$:
$$x = 8$$

Substitute $x = 8$ into equation for line #1:
$$y = -3(8) + 28$$
$$y = -24 + 28$$
$$y = 4$$

So the intersection point is $(8, 4)$


Find the intersection of Line #3 & Line #4 using elimination
---

Line #3: $y = -3x + 28$

Line #4: $y = \frac{1}{4}x + 2$

Add line #4 multiplies by 12 to line #3

$$y = -3x + 28$$
$$12y = 3x + 24$$
$$13y = 52$$
$$y = 4$$

Substitute $y = 4$ into the equation for line #1:
$$4 = -3x + 28$$
$$3x + 4 = 28$$
$$3x = 24$$
$$x = 8$$

So the intersection point is $(8, 4)$


Find the intersection of Line #5 & Line #6 using substitution
---

Line #5: $y = x + 8$

Line #6: $y = 3$

Substitute $y$ from the equation for line #6 into the equation for line #5:
$$3 = x + 8$$

Subtract 8 from both sides:
$$-5 = x$$

Substitute $x = -5$ into the equation for line #5:
$$y = -5 + 8$$
$$y = 3$$

So the intersection point is $(-5, 3)$


Find the intersection of Line #5 & Line #6 using elimination
---

Line #5: $y = x + 8$

Line #6: $y = 3$

Subtract the equation for line #6 from the equation for line #5:

$$y = x + 8$$
$$y = 3$$
$$0 = x + 5$$
$$x = -5$$

Substitute $x = -5$ into the equation for line #5:

$$y = -5 + 8$$
$$y = 3$$

So the intersection point is $(-5, 3)$


Find the intersection of Line #7 & Line #8 using substitution
---

Line #7: $y = \frac{3}{2}x + 3$

Line #8: $y = 12x - 28$

Substitute the $y$ from the equation for line #8 into the equation for line #7:
$$12x - 28 = \frac{3}{2}x + 3$$

Add $28$ to both sides:
$$12x = \frac{3}{2}x + 31$$

Subtract $\frac{3}{2}x$ from both sides:
$$10\frac{1}{2}x = 31$$

Multiply both sides by $2$:
$$21x = 62$$

Divide both sides by $21$:
$$x = \frac{62}{21}$$

Substitute $x = \frac{61}{21}$ into the equation for line #8:
$$y = 12(\frac{62}{21}) - 28$$
$$y = \frac{248}{7} - 28$$
$$y = \frac{52}{7}$$

So the intersection point is $(\frac{61}{21}, \frac{52}{7})$


Find the intersection of Line #7 & Line #8 using elimination
---

Line #7: $y = \frac{3}{2}x + 3$

Line #8: $y = 12x - 28$

Subtract the equation for line #8 from the equation for line #7:
$$y = \frac{3}{2}x + 3$$
$$y = 12x - 28$$
$$0 = -10\frac{1}{2}x + 31$$
$$10\frac{1}{2}x = 31$$
$$21x = 62$$
$$x = \frac{62}{21}$$

Substitute $x = \frac{62}{21}$ into the equation for line #8:
$$y = 12(\frac{62}{21}) - 28$$
$$y = 4(\frac{62}{7}) - \frac{196}{7}$$
$$y = \frac{248}{7} - \frac{196}{7}$$
$$y = \frac{52}{7}$$

So the intersection is $(\frac{62}{21}, \frac{52}{7})$


Find the intersection of Line #9 & Line #10 using substitution
---

Line #9: $y = 2x - 19$

Line #10: $y = -2x + 11$

Substitute the $y$ from the equation for line #10 into the equation for line #9:
$$-2x + 11 = 2x - 19$$

Add $2x$ to both sides:
$$11 = 4x - 19$$

Add $19$ to both sides:
$$30 = 4x$$
$$x = 7\frac{1}{2}$$

Substitute $x = 7\frac{1}{2}$ into the equation for line #9:
$$y = 2(7\frac{1}{2}) - 19$$
$$y = 15 - 19$$
$$y = -4$$

So the intersection is $(7\frac{1}{2}, -4)$


Find the intersection of Line #9 & Line #10 using elimination
---

Line #9: $y = 2x - 19$

Line #10: $y = -2x + 11$

Subtract the equation for line #10 from the equation for line #9:

$$y = 2x - 19$$
$$y = -2x + 11$$
$$0 = 4x - 30$$
$$4x = 30$$
$$x = 7\frac{1}{2}$$

Substitute $x = 7\frac{1}{2}$ into the equation for line #9:
$$y = 2(7\frac{1}{2}) - 19$$
$$y = 15 - 19$$
$$y = -4$$

So the intersection is $(7\frac{1}{2}, -4)$
